src/program_proof/mvcc/db_run.v
@@ -1,0 +1,59 @@
+From Perennial.program_proof.mvcc Require Import
+     txn_prelude txn_repr db_repr db_new_txn txn_run.
+
+Section program.
+Context `{!heapGS Σ, !mvcc_ghostG Σ}.
+
+Definition spec_body
+           (body : val) (txn : loc) tid r
+           (P : dbmap -> Prop) (Q : dbmap -> dbmap -> Prop)
+           (Rc : dbmap -> dbmap -> iProp Σ) (Ra : dbmap -> iProp Σ)
+           γ τ : iProp Σ :=
+  ∀ Φ,
+  own_txn txn tid r γ τ ∗ ⌜P r⌝ ∗ txnmap_ptstos τ r -∗
+  (∀ ok : bool,
+     (own_txn txn tid r γ τ ∗
+      if ok
+      then ∃ w, ⌜Q r w ∧ dom r = dom w⌝ ∗ (Rc r w ∧ Ra r) ∗ txnmap_ptstos τ w
+      else Ra r) -∗ Φ #ok) -∗
+  WP body #txn {{ v, Φ v }}.
+
+Theorem wp_DB__Run
+        (db : loc) (body : val)
+        (P : dbmap -> Prop) (Q : dbmap -> dbmap -> Prop)
+        (Rc : dbmap -> dbmap -> iProp Σ) (Ra : dbmap -> iProp Σ)
+        γ :
+  (∀ r w, (Decision (Q r w))) ->
+  is_db db γ -∗
+  {{{ ∀ txn tid r τ, spec_body body txn tid r P Q Rc Ra γ τ }}}
+  <<< ∀∀ (r : dbmap), ⌜P r⌝ ∗ dbmap_ptstos γ 1 r >>>
+    DB__Run #db body @ ↑mvccN
+  <<< ∃∃ (ok : bool) (w : dbmap), if ok then ⌜Q r w⌝ ∗ dbmap_ptstos γ 1 w else dbmap_ptstos γ 1 r >>>
+  {{{ RET #ok; if ok then Rc r w else Ra r }}}.
+Proof.
+  iIntros (Hdec) "#Hdb !>".
+  iIntros (Φ) "Hbody HAU".
+  wp_call.
+  
+  (*@ func (db *DB) Run(body func(txn *Txn) bool) bool {                      @*)
+  (*@     txn := db.NewTxn()                                                  @*)
+  (*@                                                                         @*)
+  wp_apply (wp_DB__NewTxn with "Hdb").
+  iIntros (txn) "Htxn".
+  wp_pures.
+  
+  (*@     return txn.Run(body)                                                @*)
+  (*@ }                                                                       @*)
+  wp_apply (wp_txn__Run with "[$Htxn Hbody]"); [done | done |].
+  iMod "HAU" as (r) "[[%HP Hdbpts] HAU]".
+  iModIntro.
+  iExists r.
+  iFrame.
+  iSplit; first done.
+  iIntros (ok w) "Hpost".
+  iMod ("HAU" $! ok w with "Hpost") as "HΦ".
+  iIntros "!> [Htxn HR]".
+  by iApply "HΦ".
+Qed.
+
+End program.
